some progress on weakly deterministic terms and values

SystemFD/Reduction.lean
@@ -149,10 +149,10 @@ inductive Red : Ctx Term -> Term -> Term -> Prop where
 | guard_map :
   Red Γ (.guard p (c1 ⊕ c2) b) (.guard p c1 b ⊕ .guard p c2 b)
 
-inductive RedStar : Ctx Term -> Term -> Term -> Prop where
+inductive RedStar (Γ : Ctx Term) : Term -> Term -> Prop where
 | refl : RedStar Γ x x
 | step : RedStar Γ x y -> Red Γ y z -> RedStar Γ x z
 
 
-notation:25 M:20 " ⟨ " Γ:20 " ⟩⟶⋆ " N:20 => RedStar Γ M N
-notation:25 M:20 " ⟨ " Γ:20 " ⟩⟶ " N:20 => Red Γ M N
+notation:175 M:175 " ⟨ " Γ:170 " ⟩⟶⋆ " N:170 => RedStar Γ M N
+notation:175 M:175 " ⟨ " Γ:170 " ⟩⟶ " N:170 => Red Γ M N
