SystemFD/Metatheory/Confluence.lean
@@ -1,0 +1,53 @@
+import SystemFD.Reduction
+import SystemFD.Metatheory.Canonicity
+
+
+theorem reds_trans {Γ : Ctx Term} {L M R : Term} :
+  L ⟨ Γ ⟩⟶⋆ M ->
+  (M ⟨ Γ ⟩⟶⋆ R) ->
+  L ⟨ Γ ⟩⟶⋆ R := by
+intro s1 s2
+induction s1
+assumption
+sorry
+
+theorem reds_choice_parallel {Γ : Ctx Term} {L L' R R'} :
+  L ⟨ Γ ⟩⟶⋆ R ->
+  L' ⟨ Γ ⟩⟶⋆ R' ->
+  (L ⊕ L') ⟨ Γ ⟩⟶⋆ (R ⊕ R') := by sorry
+
+
+
+theorem confluence {Γ : Ctx Term} {M v1 v2: Term} :
+  (M ⟨ Γ ⟩⟶⋆ v1) ->
+  (M ⟨ Γ ⟩⟶⋆ v2) ->
+  Val Γ v1 ->
+  Val Γ v2 ->
+  v1 = v2 := by
+sorry
+
+theorem choice_lift_red_lhs :
+  (M ⟨ Γ ⟩⟶⋆ v) ->
+  (M ⊕ N) ⟨ Γ ⟩⟶⋆ (v ⊕ N) := by
+intro h1
+induction h1
+constructor
+case _ y z _ _ ih =>
+  apply @RedStar.step Γ (M ⊕ N) (y ⊕ N) (z ⊕ N) ih
+
+
+  sorry
+
+theorem choice_reduction_unqiue {Γ : Ctx Term} {M N v: Term}:
+  (M ⟨ Γ ⟩⟶⋆ v) ->
+  (N ⟨ Γ ⟩⟶⋆ `0) ->
+  (M ⊕ N) ⟨ Γ ⟩⟶⋆ v := by
+intro h1 h2
+
+have lem1 : (M ⊕ N) ⟨ Γ ⟩⟶⋆ (M ⊕ `0) := by sorry
+have lem2 : (M ⊕ `0) ⟨ Γ ⟩⟶⋆ v := by
+  apply @RedStar.step Γ (M ⊕ `0) (v ⊕ `0) v
+  sorry
+  constructor
+
+sorry
