SystemFD/Metatheory/SemSoundness.lean
@@ -1,0 +1,60 @@
+import SystemFD.Term
+import SystemFD.Term.Subexpression
+import SystemFD.Metatheory.Canonicity
+import SystemFD.Metatheory.Confluence
+
+def saturated : Ctx Term -> Term -> Prop := sorry
+
+-- change Term.subexpr to Term.contains_variant decidable predicate
+
+inductive WDVal : Ctx Term -> Term -> Prop where
+|  WDVal :
+     Val Γ t ->
+     ¬ (Term.Subexpr `0 t) ->
+     ∀ M N, ¬ (Term.Subexpr (M ⊕ N) t) ->
+     ∀ M N P, ¬ (Term.Subexpr (.guard M P N) t) ->
+     (∀ x, Term.Subexpr #x t -> Γ.is_openm x -> saturated Γ #x) ->
+     WDVal Γ t
+
+
+inductive WDTerm : Ctx Term -> Term -> Prop where
+| WDBase :
+    (∃ v, (M ⟨ Γ ⟩⟶⋆ v) ∧  WDVal Γ v) ->
+    WDTerm Γ M
+| WDChoice1 :
+   WDTerm Γ M ->
+   (N ⟨ Γ ⟩⟶⋆ `0) ->
+   WDTerm Γ (M ⊕ N)
+| WDChoice2 :
+   WDTerm Γ N ->
+   (M ⟨ Γ ⟩⟶⋆ `0) ->
+   WDTerm Γ (M ⊕ N)
+
+-- chain
+theorem sanity :
+  WDTerm Γ M ->
+  ∃ v, (M ⟨ Γ ⟩⟶⋆ v) ∧ WDVal Γ v := by
+intro h;
+induction h
+assumption
+case _ M N h1 h2 ih =>
+  cases ih; case _ v ih =>
+  cases ih; case _ ih1 ih2 =>
+  have lem : (M ⊕ N) ⟨ Γ ⟩⟶⋆ (v ⊕ `0) := by
+    apply reds_choice_parallel ih1 h2
+  have lem2 : (v ⊕ `0) ⟨ Γ ⟩⟶⋆ v := by apply RedStar.step; (apply RedStar.refl); constructor
+  exists v
+  constructor
+  apply reds_trans lem lem2
+  assumption
+
+case _ N M h1 h2 ih =>
+  cases ih; case _ v ih =>
+  cases ih; case _ ih1 ih2 =>
+  have lem : (M ⊕ N) ⟨ Γ ⟩⟶⋆ (`0 ⊕ v) := by
+    apply reds_choice_parallel h2 ih1
+  have lem2 : (`0 ⊕ v) ⟨ Γ ⟩⟶⋆ v := by apply RedStar.step; (apply RedStar.refl); constructor
+  exists v
+  constructor
+  apply reds_trans lem lem2
+  assumption
